Datalog/Utils.lean
@@ -1,7 +1,22 @@
 def List.product (xs : List α) (len : Nat := 1) : List (List α) :=
   match len with
   | 0 => [[]]
-  | n + 1 => xs.product n |>.flatMap (fun p => xs.map (fun x => x :: p))
+  | n + 1 => xs.product n |>.flatMap (fun tup => xs.map (fun x => x :: tup))
 
+#eval [1, 2, 3].product 0
 #eval [1, 2, 3].product
 #eval [1, 2, 3].product 3
+
+theorem List.mem_product_iff (xs : List α) (len : Nat) :
+    ∀ tup, tup ∈ xs.product len ↔ tup.length = len ∧ ∀ e ∈ tup, e ∈ xs := by
+  intro tup
+  induction len generalizing tup with
+  | zero =>
+    simp [List.product]
+    grind
+  | succ n ih =>
+    constructor <;> intro h
+    · simp [List.product] at h
+      grind
+    · simp [List.product]
+      cases tup with grind
