Datalog.lean
@@ -1,1 +1,0 @@
-import Datalog.Basic
